ContextTyping/theories/PrimOpContext.v
@@ -1557,13 +1557,19 @@ Proof.
     + apply primop_graph_result_to_arg_ctx.
 Qed.
 
-Definition cons_arg1_ty : context_ty := precise_ty TNat qual_top.
-Definition cons_arg2_ty : context_ty := precise_ty TList qual_top.
-Definition cons_res_qual : type_qualifier :=
-  tqual ({[LVBound 0; LVBound 1; LVBound 2]})
-    (λ σ, ∃ x l l',
-        denote_lvar_value (lso_store σ) (vbvar 2) = Some (vconst x) ∧
-        denote_lvar_value (lso_store σ) (vbvar 1) = Some (vconst l) ∧
-        denote_lvar_value (lso_store σ) (vbvar 0) = Some (vconst l') ∧ 
-        binop_step op_cons x l l').
-Definition cons_res_ty : context_ty := over_ty TList cons_res_qual.
+Definition bin_op_arg1_ty (op : bin_op) : context_ty :=
+  over_ty (fst $ fst $ bin_op_type op) qual_top.
+
+Definition bin_op_arg2_ty (op : bin_op) : context_ty :=
+  over_ty (snd $ fst $ bin_op_type op) qual_top.
+
+Definition bin_op_res_qual (op : bin_op) (X Y : atom) : type_qualifier :=
+  tqual {[#ₗ0]}
+    (λ σ, ∃ (x y z : constant), binop_step op x y z ∧
+        lso_store σ !! LVFree X = Some (x : value) ∧
+        lso_store σ !! LVFree X = Some (y : value) ∧
+        lso_store σ !! #ₗ0 = Some (z : value)).
+
+Definition bin_op_res_ty (op : bin_op) (X Y : atom) :=
+  precise_ty (snd $ bin_op_type op) (bin_op_res_qual op X Y).
+
