CoreLang/theories/LocallyNamelessExtra.v
@@ -157,6 +157,7 @@ Proof.
   - f_equal; eauto; my_set_solver.
   - f_equal; eauto; my_set_solver.
   - f_equal; eauto; my_set_solver.
+  - f_equal; eauto; my_set_solver.
 Qed.
 
 Lemma subst_commute_tm x ux y uy e :
@@ -179,6 +180,7 @@ Proof.
     + destruct (decide (x = x0)); subst; simpl.
       * symmetry. by rewrite subst_fresh_value_proven.
       * by rewrite decide_False by done.
+  - f_equal; eauto.
   - f_equal; eauto.
   - f_equal; eauto.
   - f_equal; eauto.
@@ -215,6 +217,7 @@ Proof.
   - f_equal; eauto.
   - f_equal; eauto.
   - f_equal; eauto.
+  - f_equal; eauto.
 Qed.
 
 Lemma subst_subst_tm x ux y uy e :
@@ -235,6 +238,7 @@ Proof.
     + destruct (decide (x = x0)); subst; simpl.
       * symmetry. by rewrite subst_fresh_value_proven.
       * by rewrite decide_False by done.
+  - f_equal; eauto.
   - f_equal; eauto.
   - f_equal; eauto.
   - f_equal; eauto.
@@ -321,6 +325,8 @@ Proof.
     f_equal; eauto.
   - injection Hopen as H1 H2 H3.
     f_equal; eauto.
+  - injection Hopen as H1 H2 H3.
+    f_equal; eauto.
 Qed.
 
 Lemma open_close_var_tm_aux x e k :
@@ -344,6 +350,8 @@ Proof.
   - injection Hopen as H1 H2.
     f_equal; eauto.
   - injection Hopen as H1 H2.
+    f_equal; eauto.
+  - injection Hopen as H1 H2 H3.
     f_equal; eauto.
   - injection Hopen as H1 H2 H3.
     f_equal; eauto.
@@ -430,6 +438,7 @@ Proof.
   - f_equal; eauto; my_set_solver.
   - f_equal; eauto; my_set_solver.
   - f_equal; eauto; my_set_solver.
+  - f_equal; eauto; my_set_solver.
 Qed.
 
 Lemma subst_shadow_tm x z u e :
@@ -450,6 +459,7 @@ Proof.
   - f_equal; eauto.
   - f_equal; eauto.
   - f_equal; eauto.
+  - f_equal; eauto; my_set_solver.
   - f_equal; eauto; my_set_solver.
   - f_equal; eauto; my_set_solver.
   - f_equal; eauto; my_set_solver.
