CoreLang/theories/Sugar.v
@@ -33,6 +33,8 @@ with tm_shift (k : nat) (e : tm) : tm :=
   | tbinop op v1 v2 => tbinop op (value_shift k v1) (value_shift k v2)
   | tmatch v et ef =>
       tmatch (value_shift k v) (tm_shift k et) (tm_shift k ef)
+  | tlelim v e f =>
+      tlelim (value_shift k v) (tm_shift k e) (value_shift k f)
   end.
 
 #[global] Instance shift_value_inst : Shift value := value_shift.
@@ -128,6 +130,9 @@ Proof.
   - rewrite H by exact H2.
     rewrite H0 by exact H2.
     rewrite H1 by exact H2. reflexivity.
+  - rewrite H by exact H2.
+    rewrite H0 by exact H2.
+    rewrite H1 by exact H2. reflexivity.
 Qed.
 
 Lemma value_shift_open_value_fvar v k cutoff x :
@@ -176,6 +181,9 @@ Proof.
     rewrite H0 by exact H1. reflexivity.
   - rewrite H by exact H1.
     rewrite H0 by exact H1. reflexivity.
+  - rewrite H by exact H2.
+    rewrite H0 by exact H2.
+    rewrite H1 by exact H2. reflexivity.
   - rewrite H by exact H2.
     rewrite H0 by exact H2.
     rewrite H1 by exact H2. reflexivity.
@@ -248,6 +256,7 @@ Proof.
   - rewrite H. reflexivity.
   - rewrite H, H0. reflexivity.
   - rewrite H, H0. reflexivity.
+  - rewrite H, H0, H1. reflexivity.
   - rewrite H, H0, H1. reflexivity.
 Qed.
 
@@ -358,13 +367,13 @@ Proof.
   unfold tapp_tm.
   intros Hty.
   inversion Hty as
-    [|Γ0 Tfun Tbody ef ebody L Hef Hbody| | | |]; subst.
+    [|Γ0 Tfun Tbody ef ebody L Hef Hbody| | | | |]; subst.
   pose (x := fresh_for (L ∪ dom Γ ∪ fv_tm e ∪ {[y]})).
   assert (Hx : x ∉ L ∪ dom Γ ∪ fv_tm e ∪ {[y]})
     by (subst x; apply fresh_for_not_in).
   specialize (Hbody x ltac:(set_solver)).
   change (<[x:=Tfun]> Γ ⊢ₑ tapp (vfvar x) (vfvar y) ⋮ T) in Hbody.
-  inversion Hbody as [| | | |Γ1 s1 s2 v1 v2 Hfun Harg|]; subst.
+  inversion Hbody as [| | | |Γ1 s1 s2 v1 v2 Hfun Harg| |]; subst.
   inversion Hfun; subst.
   rewrite lookup_insert in H1.
   destruct (decide (x = x)); [|congruence].
@@ -381,7 +390,7 @@ Lemma basic_typing_tapp_tm_tlete_assoc Γ e1 e2 y T :
 Proof.
   intros Hty.
   inversion Hty as
-    [|Γ0 T1 T2 e1' e2' L He1 Hbody| | | |]; subst.
+    [|Γ0 T1 T2 e1' e2' L He1 Hbody| | | | |]; subst.
   pose (x := fresh_for (L ∪ dom Γ ∪ fv_tm e2 ∪ {[y]})).
   assert (Hx : x ∉ L ∪ dom Γ ∪ fv_tm e2 ∪ {[y]})
     by (subst x; apply fresh_for_not_in).
@@ -419,7 +428,7 @@ Proof.
   intros Hty.
   apply basic_typing_tapp_tm_fvar_inv in Hty as [Tx [Hlet Hy]].
   inversion Hlet as
-    [|Γ0 T1 T2 e1' e2' L He1 Hbody| | | |]; subst.
+    [|Γ0 T1 T2 e1' e2' L He1 Hbody| | | | |]; subst.
   eapply TT_Let with (L := L ∪ dom Γ ∪ fv_tm e2 ∪ {[y]}).
   - exact He1.
   - intros z Hz.
